---
title: "Production FUnctions"
author: "Massimiliano"
date: "20 febbraio 2017"
output: pdf_document
---

#Example of Cobb-Douglas function
======================
$$
F(K, L) = \left[\gamma K^\frac{(\sigma - 1)}{\sigma} + (1 - \gamma)L^\frac{(\sigma - 1)}{\sigma} \right]^\frac{\sigma}{\sigma - 1}
$$

#Example of CES function
=======================
$$
F(K, L) = K^\alpha L^\beta
$$

#Example of Leontief function (perfect complements)
===========================
$$
F(K, L) = min\left\{\alpha K, \beta L \right \}
$$

#CES Function
===============================
##Form
Following Chen (2011), we provide a proof of the form of CES function.
For more details on CES function, read \href{http://www.aae.wisc.edu/aae705/References/Arrow_etal_1961.pdf}{Arrow et. al (1961)}

The production function $V = F(K,L)$ in capital version can be written as 

$$
\frac{V}{L} = F\left(\frac{K}{L}, 1 \right)
$$
Let us start from $ln\frac{V}{L} = lna + blnw$

where,

$$
\begin{aligned}
  &\ \frac{V}{L} = y \\
  &\ \frac{K}{L} = k \\
  &\ MPK = f'(k) \\
  &\ MPL = f(k) - kf'(k) \\
\end{aligned}
$$
We can write

$$
lny = ln a + b ln [f(k) - kf'(k)]
$$
Solving for $f'(k)$

$$
\begin{aligned}
  &\ ln y - ln a = b ln [y - k f'(k)] \\
  &\ ln \frac{y}{a} = b ln [y - k f'(k)] \\
  &\ ln \left(\frac{y}{a} \right)^\frac{1}{b} = ln [y - k f'(k)] \\
  &\ k f'(k) = y - \left(\frac{y}{a} \right)^\frac{1}{b} \\
  &\ k f'(k) = y - \frac{y^\frac{1}{b}}{a^\frac{1}{b}} \\
  &\ f'(k) = \frac{{a^\frac{1}{b}}y - y^\frac{1}{b}}{ka^\frac{1}{b}}\\
\end{aligned}
$$
where

$$
\frac{{a^\frac{1}{b}}y - y^\frac{1}{b}}{ka^\frac{1}{b}} =
\frac{{a^\frac{-1}{b}(a^\frac{1}{b}}y - y^\frac{1}{b})}{k} =
\frac{y - a^\frac{-1}{b}y^\frac{1}{b}}{k}
$$
Setting $\alpha = a^\frac{-1}{b}$ and $\rho = \frac{1}{b} - 1$, we can write

$$
\frac{dy}{dk} = \frac{y - \alpha y^\frac{1}{b}}{k}= \frac{y(1 - \alpha y^{\frac{1}{b}-1})}{k} = \frac{y(1 - \alpha y^\rho)}{k}
$$
Becuase it is a separable differential equation, first let us separate $y$ and $k$, perform partial fraction decomposition, and take integral on both sides:

$$
\begin{aligned}
   &\ \frac{dk}{k} = \frac{dy}{y(1 - \alpha y^\rho)}\\
   &\ \frac{dk}{k} = \frac{dy}{y} + \frac{\alpha y^{\rho-1}dy}{1 - \alpha y^\rho}\\
   &\ ln k = ln y - \frac{1}{\rho} ln (1 - \alpha y^\rho) + \frac{1}{\rho} ln \beta
\end{aligned}
$$
where $ln \beta$ is a constat term after indifinite integration. Take antilog on both sides and raise the power of $\rho$ to get 

$$
k^\rho = \frac{\beta y^\rho}{1 - \alpha y^\rho}
$$
and solve for $y$

$$
\begin{aligned}
   &\ k^\rho (1 - \alpha y^\rho) = \beta y^\rho \\
   &\ k^\rho - \alpha k^\rho y^\rho = \beta y^\rho \\
   &\ k^\rho = \beta y^\rho + \alpha k^\rho y^\rho \\
   &\ k^\rho = (\beta + \alpha k^\rho)y^\rho \\
   &\ y^\rho = \frac{k^\rho}{\beta + \alpha k^\rho}\\
   &\ y = \left(\frac{k^\rho}{\beta + \alpha k^\rho} \right)^\frac{1}{\rho}\\
   &\ y = k(\beta + \alpha k^\rho)^\frac{-1}{\rho}\\
   &\ y = \left[k^{-\rho} (\beta + \alpha k^\rho)\right]^\frac{-1}{\rho}\\
   &\ y = (\beta k^{-\rho} + \alpha)^\frac{-1}{\rho}\\
\end{aligned}
$$
It can be written in the aggregate form as 

$$
F(K, L) = (\beta K^{-\rho} + \alpha L)^\frac{-1}{\rho}
$$  


#References
=======================
K. J. Arrow, H. B. Chenery, B. S. Minhas, R. M. Solow (1961). Capital-Labor Substitution and Economic Efficiency, \textit{The Review of Economics and Statistics}, Vol. 43, No. 3, pp. 225-250. 

Weijie Chen (2011). CES functions and Dixit-Stiglitz Formulation, Department of Political and Economic Studies, University of Helsinki.